Add sphinx documentation

doc/conf.py
@@ -1,0 +1,85 @@
+# Configuration file for the Sphinx documentation builder.
+#
+# This file only contains a selection of the most common options. For a full
+# list see the documentation:
+# https://www.sphinx-doc.org/en/master/usage/configuration.html
+
+# -- Path setup --------------------------------------------------------------
+
+# If extensions (or modules to document with autodoc) are in another directory,
+# add these directories to sys.path here. If the directory is relative to the
+# documentation root, use os.path.abspath to make it absolute, like shown here.
+#
+# import os
+# import sys
+# sys.path.insert(0, os.path.abspath('.'))
+
+
+# -- Project information -----------------------------------------------------
+
+project = 'Vericert'
+copyright = '2022  Yann Herklotz, John Wickerson'
+author = 'Yann Herklotz, John Wickerson'
+
+# The full version, including alpha/beta/rc tags
+release = 'v1.2.2'
+
+
+# -- General configuration ---------------------------------------------------
+
+# Add any Sphinx extension module names here, as strings. They can be
+# extensions coming with Sphinx (named 'sphinx.ext.*') or your custom
+# ones.
+extensions = [ "alectryon.sphinx" ]
+
+# Add any paths that contain templates here, relative to this directory.
+templates_path = ['_templates']
+
+# List of patterns, relative to source directory, that match files and
+# directories to ignore when looking for source files.
+# This pattern also affects html_static_path and html_extra_path.
+exclude_patterns = ['_build', 'Thumbs.db', '.DS_Store']
+
+pygments_style = "emacs"
+
+
+# -- Options for HTML output -------------------------------------------------
+
+# The theme to use for HTML and HTML Help pages.  See the documentation for
+# a list of builtin themes.
+#
+html_theme = 'alabaster'
+
+# Add any paths that contain custom static files (such as style sheets) here,
+# relative to this directory. They are copied after the builtin static files,
+# so a file named "default.css" will overwrite the builtin "default.css".
+html_static_path = ['_static']
+
+html_css_files = [
+    'css/custom.css',
+]
+
+
+# -- LaTeX configuration -----------------------------------------------------
+
+latex_engine = "xelatex"
+
+
+# -- Alectryon configuration -------------------------------------------------
+
+import alectryon.docutils
+alectryon.docutils.CACHE_DIRECTORY = "_build/alectryon/"
+alectryon.docutils.LONG_LINE_THRESHOLD = 80
+
+alectryon.docutils.AlectryonTransform.DRIVER_ARGS["sertop"] = [
+    "-R" "../src,vericert",
+    "-R" "../lib/CompCert/lib,compcert.lib",
+    "-R" "../lib/CompCert/common,compcert.common",
+    "-R" "../lib/CompCert/verilog,compcert.verilog",
+    "-R" "../lib/CompCert/backend,compcert.backend",
+    "-R" "../lib/CompCert/cfrontend,compcert.cfrontend",
+    "-R" "../lib/CompCert/driver,compcert.driver",
+    "-R" "../lib/CompCert/cparser,compcert.cparser",
+    "-R" "../lib/CompCert/flocq,Flocq",
+    "-R" "../lib/CompCert/MenhirLib,MenhirLib"
+]
