doc/index.rst
@@ -1,0 +1,26 @@
+.. Vericert documentation master file, created by
+   sphinx-quickstart on Sat Mar 26 18:15:40 2022.
+   You can adapt this file completely to your liking, but it should at least
+   contain the root `toctree` directive.
+
+Vericert's Documentation
+========================
+
+.. toctree::
+   :maxdepth: 2
+   :caption: Content:
+
+   vericert
+
+.. toctree::
+   :maxdepth: 1
+   :caption: Sources:
+
+   src/Compiler
+   src/hls/RTLBlockInstr
+
+Indices
+==================
+
+* :ref:`genindex`
+* :ref:`search`
