doc/vericert.rst
@@ -1,0 +1,530 @@
+===============
+Vericert Manual
+===============
+
+
+Introduction
+------------
+
+Vericert translates C code into a hardware description language called Verilog, which can then be
+synthesised into hardware, to be placed onto a field-programmable gate array (FPGA) or
+application-specific integrated circuit (ASIC).
+
+.. _fig:design:
+
+.. figure:: /_static/images/toolflow.png
+
+    Current design of Vericert, where HTL is an intermediate language representing a finite state
+    machine with data-path (FSMD) and Verilog is the target language.
+
+The design shown in Figure `fig:design`_ shows how Vericert leverages an existing verified C
+compiler called `CompCert <https://compcert.org/compcert-C.html>`_ to perform this translation.
+
+.. index:: vericert
+
+.. _building:
+
+Building Vericert
+-----------------
+
+
+Testing
+~~~~~~~
+
+To test out ``vericert`` you can try the following examples which are in the test folder using the
+following:
+
+.. code:: shell
+
+    ./bin/vericert test/loop.c -o loop.v
+    ./bin/vericert test/conditional.c -o conditional.v
+    ./bin/vericert test/add.c -o add.v
+
+Or by running the test suite using the following command:
+
+.. code:: shell
+
+    make test
+
+.. _using-vericert:
+
+.. index:: vericert
+
+Using Vericert
+--------------
+
+Vericert can be used to translate a subset of C into Verilog.  As a simple example, consider the
+following C file (``main.c``):
+
+.. code:: C
+
+    void matrix_multiply(int first[2][2], int second[2][2], int multiply[2][2]) {
+        int sum = 0;
+        for (int c = 0; c < 2; c++) {
+            for (int d = 0; d < 2; d++) {
+                for (int k = 0; k < 2; k++) {
+                    sum = sum + first[c][k]*second[k][d];
+                }
+                multiply[c][d] = sum;
+                sum = 0;
+            }
+        }
+    }
+
+    int main() {
+        int f[2][2] = {{1, 2}, {3, 4}};
+        int s[2][2] = {{5, 6}, {7, 8}};
+        int m[2][2] = {{0, 0}, {0, 0}};
+
+        matrix_multiply(f, s, m);
+        return m[1][1];
+    }
+
+It can be compiled using the following command, assuming that vericert is somewhere on the path.
+
+.. code:: shell
+
+    vericert main.c -o main.v
+
+The Verilog file contains a top-level test-bench, which can be given to any Verilog simulator to
+simulate the hardware, which should give the same result as executing the C code.  Using `Icarus
+Verilog <http://iverilog.icarus.com/>`_ as an example:
+
+.. code:: shell
+
+    iverilog -o main_v main.v
+
+When executing, it should therefore print the following:
+
+.. code:: shell
+
+    $ ./main_v
+    finished: 50
+
+This gives the same result as executing the C in the following way:
+
+.. code:: shell
+
+    $ gcc -o main_c main.c
+    $ ./main_c
+    $ echo $?
+    50
+
+Man pages
+~~~~~~~~~
+
+.. _unreleased-features:
+
+Unreleased Features
+-------------------
+
+The following are unreleased features in Vericert that are currently being worked on and have not
+been completely proven correct yet.  Currently this includes features such as:
+
+- `scheduling`_,
+
+- `operation-chaining`_,
+
+- `if-conversion`_, and
+
+- `functions`_.
+
+This page gives some preliminary information on how the features are implemented and how the proofs
+for the features are being done.  Once these features are properly implemented, they will be added
+to the proper documentation.
+
+.. _scheduling:
+
+Scheduling
+~~~~~~~~~~
+
+Scheduling is an optimisation which is used to run various instructions in parallel that are
+independent to each other.
+
+.. _operation-chaining:
+
+Operation Chaining
+~~~~~~~~~~~~~~~~~~
+
+Operation chaining is an optimisation that can be added on to scheduling and allows for the
+sequential execution of instructions in a clock cycle, while executing other instructions in
+parallel in the same clock cycle.
+
+.. _if-conversion:
+
+If-conversion
+~~~~~~~~~~~~~
+
+If-conversion is an optimisation which can turn code with simple control flow into a single block
+(called a hyper-block), using predicated instructions.
+
+.. _functions:
+
+Functions
+~~~~~~~~~
+
+Functions are currently only inlined in Vericert, however, we are working on a proper interface to
+integrate function calls into the hardware.
+
+.. _coq-style-guide:
+
+Coq Style Guide
+---------------
+
+This style guide was taken from `Silveroak <https://github.com/project-oak/silveroak>`_, it outlines
+code style for Coq code in this repository. There are certainly other valid strategies and opinions
+on Coq code style; this is laid out purely in the name of consistency. For a visual example of the
+style, see the `example`_ at the bottom of this file.
+
+.. _code-organization:
+
+Code organization
+~~~~~~~~~~~~~~~~~
+
+.. _legal-banner:
+
+Legal banner
+^^^^^^^^^^^^
+
+- Files should begin with a copyright/license banner, as shown in the example above.
+
+.. _import-statements:
+
+Import statements
+^^^^^^^^^^^^^^^^^
+
+- ``Require Import`` statements should all go at the top of the file, followed by file-wide ``Import``
+  statements.
+
+  - =Import=s often contain notations or typeclass instances that might override notations or
+    instances from another library, so it’s nice to highlight them separately.
+
+- One ``Require Import`` statement per line; it’s easier to scan that way.
+
+- ``Require Import`` statements should use “fully-qualified” names (e.g. ``Require Import
+  Coq.ZArith.ZArith`` instead of ``Require Import ZArith``).
+
+  - Use the ``Locate`` command to find the fully-qualified name!
+
+- ``Require Import``’s should go in the following order:
+
+  1. Standard library dependencies (start with ``Coq.``)
+
+  2. External dependencies (anything outside the current project)
+
+  3. Same-project dependencies
+
+- ``Require Import``’s with the same root library (the name before the first ``.``) should be
+  grouped together. Within each root-library group, they should be in alphabetical order (so
+  ``Coq.Lists.List`` before ``Coq.ZArith.ZArith``).
+
+.. _notations-and-scopes:
+
+Notations and scopes
+^^^^^^^^^^^^^^^^^^^^
+
+- Any file-wide ``Local Open Scope``’s should come immediately after the =Import=s (see example).
+
+  - Always use ``Local Open Scope``; just ``Open Scope`` will sneakily open the scope for those who
+    import your file.
+
+- Put notations in their own separate modules or files, so that those who import your file can
+  choose whether or not they want the notations.
+
+  - Conflicting notations can cause a lot of headache, so it comes in very handy to leave this
+    flexibility!
+
+.. _formatting:
+
+Formatting
+~~~~~~~~~~
+
+.. _line-length:
+
+Line length
+^^^^^^^^^^^
+
+- Maximum line length 80 characters.
+
+  - Many Coq IDE setups divide the screen in half vertically and use only half to display source
+    code, so more than 80 characters can be genuinely hard to read on a laptop.
+
+.. _whitespace-and-indentation:
+
+Whitespace and indentation
+^^^^^^^^^^^^^^^^^^^^^^^^^^
+
+- No trailing whitespace.
+
+- Spaces, not tabs.
+
+- Files should end with a newline.
+
+  - Many editors do this automatically on save.
+
+- Colons may be either “English-spaced”, with no space before the colon and one space after (``x:
+  nat``) or “French-spaced”, with one space before and after (``x : nat``).
+
+- Default indentation is 2 spaces.
+
+  - Keeping this small prevents complex proofs from being indented ridiculously far, and matches IDE
+    defaults.
+
+- Use 2-space indents if inserting a line break immediately after:
+
+  - ``Proof.``
+
+  - ``fun <...> =>``
+
+  - ``forall <...>,``
+
+  - ``exists <....>,``
+
+- The style for indenting arguments in function application depends on where you make a line
+  break. If you make the line break immediately after the function name, use a 2-space
+  indent. However, if you make it after one or more arguments, align the next line with the first
+  argument:
+
+  .. code:: coq
+
+      (Z.pow
+         1 2)
+      (Z.pow 1 2 3
+             4 5 6)
+
+- ``Inductive`` cases should not be indented. Example:
+
+  .. code:: coq
+
+      Inductive Foo : Type :=
+      | FooA : Foo
+      | FooB : Foo
+      .
+
+- ``match`` or ``lazymatch`` cases should line up with the “m” in ``match`` or “l” in ``lazymatch``,
+  as in the following examples:
+
+  .. code:: coq
+
+      match x with
+      | 3 => true
+      | _ => false
+      end.
+
+      lazymatch x with
+      | 3 => idtac
+      | _ => fail "Not equal to 3:" x
+      end.
+
+      repeat match goal with
+             | _ => progress subst
+             | _ => reflexivity
+             end.
+
+      do 2 lazymatch goal with
+           | |- context [eq] => idtac
+           end.
+
+.. _definitions-and-fixpoints:
+
+Definitions and Fixpoints
+~~~~~~~~~~~~~~~~~~~~~~~~~
+
+- It’s okay to leave the return type of ``Definition``’s and ``Fixpoint``’s implicit
+  (e.g. ``Definition x := 5`` instead of ``Definition x : nat := 5``) when the type is very simple
+  or obvious (for instance, the definition is in a file which deals exclusively with operations on
+  ``Z``).
+
+.. _inductives:
+
+Inductives
+~~~~~~~~~~
+
+- The ``.`` ending an ``Inductive`` can be either on the same line as the last case or on its own
+  line immediately below. That is, both of the following are acceptable:
+
+  .. code:: coq
+
+      Inductive Foo : Type :=
+      | FooA : Foo
+      | FooB : Foo
+      .
+      Inductive Foo : Type :=
+      | FooA : Foo
+      | FooB : Foo.
+
+.. _lemmatheorem-statements:
+
+Lemma/Theorem statements
+~~~~~~~~~~~~~~~~~~~~~~~~
+
+- Generally, use ``Theorem`` for the most important, top-level facts you prove and ``Lemma`` for
+  everything else.
+
+- Insert a line break after the colon in the lemma statement.
+
+- Insert a line break after the comma for ``forall`` or ``exist`` quantifiers.
+
+- Implication arrows (``->``) should share a line with the previous hypothesis, not the following
+  one.
+
+- There is no need to make a line break after every ``->``; short preconditions may share a line.
+
+.. _proofs-and-tactics:
+
+Proofs and tactics
+~~~~~~~~~~~~~~~~~~
+
+- Use the ``Proof`` command (lined up vertically with ``Lemma`` or ``Theorem`` it corresponds to) to
+  open a proof, and indent the first line after it 2 spaces.
+
+- Very small proofs (where ``Proof. <tactics> Qed.`` is <= 80 characters) can go all in one line.
+
+- When ending a proof, align the ending statement (``Qed``, ``Admitted``, etc.) with ``Proof``.
+
+- Avoid referring to autogenerated names (e.g. ``H0``, ``n0``). It’s okay to let Coq generate these
+  names, but you should not explicitly refer to them in your proof. So ``intros; my_solver`` is
+  fine, but ``intros; apply H1; my_solver`` is not fine.
+
+  - You can force a non-autogenerated name by either putting the variable before the colon in the
+    lemma statement (``Lemma foo x : ...`` instead of ``Lemma foo : forall x, ...``), or by passing
+    arguments to ``intros`` (e.g. ``intros ? x`` to name the second argument ``x``)
+
+- This way, the proof won’t break when new hypotheses are added or autogenerated variable names
+  change.
+
+- Use curly braces ``{}`` for subgoals, instead of bullets.
+
+- *Never write tactics with more than one subgoal focused.* This can make the proof very confusing
+  to step through! If you have more than one subgoal, use curly braces.
+
+- Consider adding a comment after the opening curly brace that explains what case you’re in (see
+  example).
+
+  - This is not necessary for small subgoals but can help show the major lines of reasoning in large
+    proofs.
+
+- If invoking a tactic that is expected to return multiple subgoals, use ``[ | ... | ]`` before the
+  ``.`` to explicitly specify how many subgoals you expect.
+
+  - Examples: ``split; [ | ].`` ``induction z; [ | | ].``
+
+  - This helps make code more maintainable, because it fails immediately if your tactic no longer
+    solves as many subgoals as expected (or unexpectedly solves more).
+
+- If invoking a string of tactics (composed by ``;``) that will break the goal into multiple
+  subgoals and then solve all but one, still use ``[ ]`` to enforce that all but one goal is solved.
+
+  - Example: ``split; try lia; [ ]``.
+
+- Tactics that consist only of ``repeat``-ing a procedure (e.g. ``repeat match``, ``repeat first``)
+  should factor out a single step of that procedure a separate tactic called ``<tactic name>_step``,
+  because the single-step version is much easier to debug. For instance:
+
+  .. code:: coq
+
+      Ltac crush_step :=
+        match goal with
+        | _ => progress subst
+        | _ => reflexivity
+        end.
+      Ltac crush := repeat crush_step.
+
+.. _naming:
+
+Naming
+~~~~~~
+
+- Helper proofs about standard library datatypes should go in a module that is named to match the
+  standard library module (see example).
+
+  - This makes the helper proofs look like standard-library ones, which is helpful for categorizing
+    them if they’re genuinely at the standard-library level of abstraction.
+
+- Names of modules should start with capital letters.
+
+- Names of inductives and their constructors should start with capital letters.
+
+- Names of other definitions/lemmas should be snake case.
+
+.. _example:
+
+Example
+~~~~~~~
+
+A small standalone Coq file that exhibits many of the style points.
+
+.. code:: coq
+
+    (*
+     * Vericert: Verified high-level synthesis.
+     * Copyright (C) 2021 Name <email@example.com>
+     *
+     * <License...>
+     *)
+
+      Require Import Coq.Lists.List.
+      Require Import Coq.micromega.Lia.
+      Require Import Coq.ZArith.ZArith.
+      Import ListNotations.
+      Local Open Scope Z_scope.
+
+      (* Helper proofs about standard library integers (Z) go within [Module Z] so
+         that they match standard-library Z lemmas when used. *)
+      Module Z.
+        Lemma pow_3_r x : x ^ 3 = x * x * x.
+        Proof. lia. Qed. (* very short proofs can go all on one line *)
+
+        Lemma pow_4_r x : x ^ 4 = x * x * x * x.
+        Proof.
+          change 4 with (Z.succ (Z.succ (Z.succ (Z.succ 0)))).
+          repeat match goal with
+                 | _ => rewrite Z.pow_1_r
+                 | _ => rewrite Z.pow_succ_r by lia
+                 | |- context [x * (?a * ?b)] =>
+                   replace (x * (a * b)) with (a * b * x) by lia
+                 | _ => reflexivity
+                 end.
+        Qed.
+      End Z.
+      (* Now we can access the lemmas above as Z.pow_3_r and Z.pow_4_r, as if they
+         were in the ZArith library! *)
+
+      Definition bar (x y : Z) := x ^ (y + 1).
+
+      (* example with a painfully manual proof to show case formatting *)
+      Lemma bar_upper_bound :
+        forall x y a,
+          0 <= x <= a -> 0 <= y ->
+          0 <= bar x y <= a ^ (y + 1).
+      Proof.
+        (* avoid referencing autogenerated names by explicitly naming variables *)
+        intros x y a Hx Hy. revert y Hy x a Hx.
+        (* explicitly indicate # subgoals with [ | ... | ] if > 1 *)
+        cbv [bar]; refine (natlike_ind _ _ _); [ | ].
+        { (* y = 0 *)
+          intros; lia. }
+        { (* y = Z.succ _ *)
+          intros.
+          rewrite Z.add_succ_l, Z.pow_succ_r by lia.
+          split.
+          { (* 0 <= bar x y *)
+            apply Z.mul_nonneg_nonneg; [ lia | ].
+            apply Z.pow_nonneg; lia. }
+          { (* bar x y < a ^ y *)
+            rewrite Z.pow_succ_r by lia.
+            apply Z.mul_le_mono_nonneg; try lia;
+              [ apply Z.pow_nonneg; lia | ].
+            (* For more flexible proofs, use match statements to find hypotheses
+               rather than referring to them by autogenerated names like H0. In this
+               case, we'll take any hypothesis that applies to and then solves the
+               goal. *)
+            match goal with H : _ |- _ => apply H; solve [auto] end. } }
+      Qed.
+
+      (* Put notations in a separate module or file so that importers can
+         decide whether or not to use them. *)
+      Module BarNotations.
+        Infix "#" := bar (at level 40) : Z_scope.
+        Notation "x '##'" := (bar x x) (at level 40) : Z_scope.
+      End BarNotations.
